formal/isabelle/TRUST12_OBSTRUCTIONS/TRUST_Accounting_Invariant_Obstruction.thy
@@ -1,0 +1,97 @@
+(*
+  A typed obstruction to promoting the accounting invariant to a regulatory-step
+  invariant.  The state below satisfies accounting_state_wf, but carries a
+  malformed freeze head that the accounting predicate deliberately does not
+  constrain.  A fully admitted FREEZE can therefore separate the custody action
+  from its case head.  This is an ill-formed-state counterexample, not a claim
+  that the state is reachable from native_initial_state.
+*)
+
+theory TRUST_Accounting_Invariant_Obstruction
+  imports TRUST_State_Invariants
+begin
+
+definition obstruction_binding :: compositional_binding where
+  "obstruction_binding =
+    \<lparr>binding_endpoint = 0, binding_code_id = 0, binding_configuration = 0,
+     binding_schema = 0, binding_epoch = 1, binding_hash = 0\<rparr>"
+
+definition obstruction_seize :: trust_forward_command where
+  "obstruction_seize =
+    \<lparr>forward_domain = 1, forward_action_id = 1, forward_action = Legal_Seize,
+     forward_subject = 1, forward_source = 1, forward_destination = 2,
+     forward_custodian = 2, forward_amount = 1, forward_case = 1,
+     forward_dependency_root = 0, forward_dependency_epoch = 1,
+     forward_provenance_commitment = 1, forward_settlement_commitment = 0,
+     forward_proceeds_commitment = 0, forward_entitlement_commitment = 0,
+     forward_authority_ref = 1, forward_authority_epoch = 1, forward_nonce = 1,
+     forward_valid_after = 0, forward_valid_before = 2\<rparr>"
+
+definition obstruction_freeze :: trust_forward_command where
+  "obstruction_freeze = obstruction_seize
+    \<lparr>forward_action := Legal_Freeze, forward_action_id := 2, forward_nonce := 2,
+     forward_destination := 0, forward_custodian := 0\<rparr>"
+
+definition obstruction_receipt :: "trust_forward_command \<Rightarrow> compositional_receipt" where
+  "obstruction_receipt command =
+    \<lparr>compositional_receipt_kind = Receipt_Action,
+     compositional_command_id = forward_action_id command,
+     compositional_command_kind = solidity_action_code (forward_action command),
+     compositional_parent_command_id = 0,
+     compositional_subject = forward_subject command,
+     compositional_source = forward_source command,
+     compositional_destination = forward_destination command,
+     compositional_amount = forward_amount command,
+     compositional_case = forward_case command,
+     compositional_authority_ref = forward_authority_ref command,
+     compositional_dependency_root = forward_dependency_root command,
+     compositional_provenance_commitment = forward_provenance_commitment command,
+     compositional_assessment_evidence = 1,
+     compositional_pre_observation = 0, compositional_post_observation = 0,
+     compositional_external_commitment = forward_external_commitment command,
+     compositional_receipt_hash = forward_action_id command\<rparr>"
+
+definition obstruction_witness :: "trust_forward_command \<Rightarrow> trust_success_witness" where
+  "obstruction_witness command =
+    \<lparr>witness_command_hash = forward_action_id command, witness_evidence_hash = 1,
+     witness_receipt = obstruction_receipt command\<rparr>"
+
+definition obstruction_initial :: trust_compositional_state where
+  "obstruction_initial =
+    native_initial_state 1 1 1 1 (\<lambda>_. obstruction_binding) 0"
+
+definition obstruction_seized :: trust_compositional_state where
+  "obstruction_seized = forward_success_state obstruction_initial obstruction_seize
+    (obstruction_witness obstruction_seize)"
+
+definition obstruction_state :: trust_compositional_state where
+  "obstruction_state = obstruction_seized\<lparr>freeze_heads :=
+    (\<lambda>_. empty_head)(1 := \<lparr>head_action = Some 1, head_generation = 1\<rparr>)\<rparr>"
+
+lemmas obstruction_compute =
+  obstruction_initial_def native_initial_state_def obstruction_seized_def obstruction_state_def
+  obstruction_seize_def obstruction_freeze_def obstruction_witness_def obstruction_receipt_def
+  forward_success_state_def base_forward_success_def forward_action_record_def
+  opened_custody_def empty_case_def empty_head_def move_balance_def Let_def
+
+theorem accounting_wf_allows_the_malformed_head:
+  "accounting_state_wf {1, 2} {1} obstruction_state"
+  by (auto simp: accounting_state_wf_def balance_wf_def case_scope_def custody_consistent_def
+      active_custody_sum_def custody_case_wf_def open_case_def obstruction_compute)
+
+theorem malformed_head_still_admits_a_freeze:
+  "forward_admitted obstruction_state 1 1 obstruction_freeze
+    (obstruction_witness obstruction_freeze)"
+  by (simp add: forward_admitted_def forward_shape_wf_def forward_fresh_def forward_nonce_key_def
+      forward_authorized_def authority_admits_def forward_current_dependency_def forward_in_window_def
+      within_window_def receipt_matches_forward_def overlay_shape_def no_disposition_commitments_def
+      overlay_admissible_def terminal_case_def forward_external_commitment_def obstruction_compute)
+
+theorem accounting_wf_is_not_preserved_by_every_admitted_forward:
+  "\<not> accounting_state_wf {1, 2} {1}
+    (forward_success_state obstruction_state obstruction_freeze
+      (obstruction_witness obstruction_freeze))"
+  by (simp add: accounting_state_wf_def custody_case_wf_def open_case_def
+      obstruction_compute opened_overlay_def)
+
+end
